code/experimental/rsapss/Hacl.Test.Bignum.fst
@@ -1,0 +1,137 @@
+module Hacl.Test.Bignum
+
+open FStar.HyperStack
+open FStar.HyperStack.ST
+open FStar.Mul
+
+open LowStar.Buffer
+
+open Lib.IntTypes
+open Lib.Buffer
+
+open Hacl.Impl.Bignum.Core
+open Hacl.Impl.Bignum.Convert
+open Hacl.Impl.Bignum.Comparison
+open Hacl.Impl.Bignum.Addition
+
+
+inline_for_extraction unfold noextract
+val print_str: string -> ST unit (requires fun _ -> true) (ensures fun h0 _ h1 -> h0 == h1)
+let print_str x = C.String.print (C.String.of_literal x)
+
+inline_for_extraction unfold noextract
+val print_strln: string -> ST unit (requires fun _ -> true) (ensures fun h0 _ h1 -> h0 == h1)
+let print_strln x = print_str (x ^ "\n")
+
+inline_for_extraction unfold noextract
+val print_bool: b:bool -> ST unit (requires fun _ -> true) (ensures fun h0 _ h1 -> h0 == h1)
+let print_bool b =
+  C.String.print (if b then C.String.of_literal "true\n" else C.String.of_literal "false\n")
+
+
+
+inline_for_extraction noextract
+val test_comparison_gen:
+     a:snat
+  -> b:snat{b <= a}
+  -> St unit
+let test_comparison_gen a b =
+  let less_exp = normalize_term (a < b) in
+  let eq_exp = normalize_term (a = b) in
+
+  admit();
+
+  let bn_a: lbignum (nat_bytes_num a) = nat_to_bignum_exact a in
+  let bn_b: lbignum (nat_bytes_num b) = nat_to_bignum_exact b in
+
+  let less_res = bn_is_less bn_a bn_b in
+  let eq_res = bn_is_equal bn_a bn_b in
+
+  let res = (less_res = less_exp && eq_res = eq_exp) in
+  if res then print_strln " * Success" else print_strln " * Failed"
+
+inline_for_extraction noextract
+val test_eq_representation:
+     a:snat{v (nat_bytes_num a) + 5 < max_size_t}
+  -> Stack unit (requires fun _ -> true) (ensures fun _ _ _ -> true)
+let test_eq_representation a =
+  push_frame();
+
+  [@inline_let]
+  let aLen = nat_bytes_num a in
+  [@inline_let]
+  let bLen = nat_bytes_num a +! 1ul in
+  [@inline_let]
+  let cLen = nat_bytes_num a +! 5ul in
+
+  let bn_a: lbignum aLen = nat_to_bignum_exact a in
+  let bn_b: lbignum bLen = nat_to_bignum a in
+  let bn_c: lbignum bLen = nat_to_bignum a in
+
+  assert_norm (v aLen > 0);
+  assert_norm (v bLen > 0);
+  assert_norm (v aLen <= v bLen);
+  let res = bn_is_equal bn_b bn_a in
+   if res then print_strln " * Success" else print_strln " * Failed";
+  pop_frame()
+
+val test_comparison: unit -> St unit
+let test_comparison _ =
+  C.String.print (C.String.of_literal "Testing comparison\n");
+  push_frame();
+
+  test_comparison_gen 0 0;
+  test_comparison_gen 1 0;
+  test_comparison_gen 12345 0;
+  test_comparison_gen 12345 12345;
+  test_comparison_gen 18446744073709551618 18446744073709551618;
+  test_comparison_gen 18446744073709551618 18446744073709551617;
+
+  C.String.print (C.String.of_literal "...leading zeroes tests:\n");
+
+  test_eq_representation 0;
+  test_eq_representation 1;
+  test_eq_representation 100;
+  test_eq_representation 10000000000000000000000000;
+
+  pop_frame()
+
+inline_for_extraction noextract
+val test_addition_gen:
+     a:snat
+  -> b:snat{b <= a}
+  -> St unit
+let test_addition_gen a b =
+  admit();
+  let bn_a   = nat_to_bignum_exact a in
+  let bn_b   = nat_to_bignum_exact b in
+  let bn_res = nat_to_bignum_exact (normalize_term (b+a)) in
+  let bn_c   = nat_to_bignum_exact (normalize_term (b+a)) in
+
+  bn_add_full bn_a bn_b bn_res;
+  let res = bn_is_equal bn_c bn_res in
+  if res then print_strln " * Success" else print_strln " * Failed"
+
+
+val test_addition: unit -> St unit
+let test_addition _ =
+  C.String.print (C.String.of_literal "Testing addition \n");
+  push_frame();
+
+  test_addition_gen 0 0;
+  test_addition_gen 1 0;
+  test_addition_gen 12345 0;
+  test_addition_gen 10 5;
+  test_addition_gen 10000000000 5;
+  test_addition_gen
+    111111111111111111111111111111
+    18446744073709551618;
+
+  pop_frame()
+
+val testBignum: unit -> St unit
+let testBignum _ =
+  C.String.print (C.String.of_literal "Bignum tests: \n");
+  test_comparison ();
+  test_addition ();
+  C.String.print (C.String.of_literal "Bignum tests are done \n\n")
